completely rethought interpreter tests

tests/lustre_programs.v
@@ -1,43 +1,181 @@
 From Stdlib Require Import Strings.String.
 
-(* Lustre programs to test the interpreter *)
-Definition prog1 : string :=
+(** * Lustre programs
+  A suite of Lustre programs to test the interpreter, showcasing very supported construct in our AST, 
+  multi-node and function calls, and why there is a two-phase evaluator (computing outputs, then commiting
+  the state).
+*)
+
+(** ** Baseline
+  Pure compinational identity, showcasing our types.
+*)
+Definition id_int : string :=
+  "node id(x:int) returns (y:int);
+  let
+    y = x;
+  tel".
+
+Definition id_bool : string :=
+  "node id(b:bool) returns (c:bool);
+  let
+    c = b;
+  tel".
+
+(** ** Constants, unary operations and binary operations
+*)
+Definition opp : string :=
+  "node opp(x:int) returns (y:int);
+  let
+    y = -x;
+  tel".
+
+Definition neg : string :=
+  "node neg(b:bool) returns (c:bool);
+  let
+    c = not b;
+  tel".
+
+Definition add : string :=
   "node add(x:int; y:int) returns (z:int);
    let
      z = x + y;
    tel".
 
-Definition prog2 : string :=
-  "node substract(x:int; y:int) returns (w:int);
+Definition substract : string :=
+  "node substract(x:int; y:int) returns (z:int);
   let
-    w = x - y; 
+    z = x - y; 
   tel".
 
-Definition prog3 : string :=
+Definition mult : string :=
   "node mult(x:int; y:int) returns (z:int);
    let
      z = x * y;
    tel".
 
-Definition prog4 : string :=
+Definition div : string :=
   "node div(x:int; y:int) returns (z:int);
    let
      z = x / y;
    tel".
 
-Definition prog5 : string :=
+Definition mod3 : string :=
   "node mod3(x:int) returns (m:int);
    let
      m = x % 3;
    tel".
 
-Definition prog6 : string :=
+Definition arith : string :=
+  "node arith (x:int; y:int) returns (a:int; m:int);
+  let
+    a = (x + y) * 2;
+    m = a % 5;
+  tel".
+
+Definition less_than : string :=
+  "node lt(x:int; y:int) returns (r:bool);
+  let
+    r = x < y;
+  tel".
+
+Definition logic : string :=
+  "node logic(b:bool; c:bool) returns (d:bool; e:bool);
+  let
+    d = b and c;
+    e = b xor c;
+  tel".
+
+(** ** Branching
+*)
+Definition if_then_else : string :=
+  "node abs(x:int) returns (y:int);
+  let
+    y = if x < 0 then -x else x;
+  tel".
+
+(** Two-phased node evaluation
+*)
+Definition pre_arrow : string :=
+  "node pre_arrow(x:int) returns (y:int);
+  let
+    y = 0 -> pre x;
+  tel".
+
+Definition count : string :=
+  "node counter() returns (c:int);
+  let
+    c = 0 fby (c + 1);
+  tel".
+
+Definition simult : string :=
+  "node simult() returns (x:int; y:int);
+  let
+    x = 0 fby (x + 1);
+    y = x + 10;
+  tel".
+
+(** ** Multiple outputs and multiple left-hand-side equation shape
+*)
+Definition two_out : string :=
+  "node two_out(x:int) returns (y:int; z:int);
+  let
+    (y, z) = (x, x+1);
+    -- z = x + 1;
+  tel".
+
+(** ** Clocks
+*)
+Definition when : string :=
+  "node gate(x:int; clk:bool) returns (y:int);
+  let
+    y = x when clk;
+  tel".
+
+Definition merge : string :=
+  "node choose(x:int; clk:bool) returns (y:int);
+  let
+    y = merge clk x (0 - x);
+  tel".
+
+Definition current : string :=
+  "node hold_last(x:int; clk:bool) returns (y:int);
+  let
+    y = current (x when clk);
+  tel".
+
+(** **  Calls
+*)
+Definition fun_def : string :=
+  "function add1(x:int) returns (y:int);
+  let
+    y = x + 1;
+  tel
+
+  node main(x:int) returns (z:int);
+  let
+    z = add1(x);
+  tel".
+
+Definition node_call : string :=
+  "node inc(x:int) returns (y:int);
+  let
+    y = x + 1;
+  tel
+
+  node main(x:int) returns (z:int);
+  let
+    z = inc(x);
+  tel".
+
+(** ** Examples from the course
+*)
+Definition raising_edge : string :=
   "node redge(b : bool) returns (edge : bool);
   let
     edge = false -> (b and not (pre b));
   tel".
 
-Definition prog7 : string :=
+Definition alternating_count : string :=
   "node mod_count(m : int) returns (y : int);
   var py : int;
   let
