tests/lustre_traces.v
@@ -1,0 +1,54 @@
+From Stdlib Require Import Strings.String Lists.List ZArith.
+Import ListNotations.
+
+(** * Traces for initializing the input
+*)
+
+(** ** Boolean traces
+*)
+Definition trace_bool_1 : list bool :=
+  [true;true;true;true;false;false;false;false;true;true;true;true;false;false;false;false].
+
+Definition trace_bool_2 : list bool :=
+  [true;false;true;false;true;false;true;false;true;false;true;false;true;false;true;false].
+
+Definition trace_bool_3 : list bool :=
+  [true;true;false;false;true;true;false;false;true;true;false;false;true;true;false;false].
+
+(* trace_tf_count-1 *)
+Definition trace_tf_count_1 : list bool :=
+  [true;true;true;false;false;false;false;true;true;true;true;false;false;false;true;true].
+
+(* trace_tf_count-2 *)
+Definition trace_tf_count_2 : list bool :=
+  [true;true;true;true;true;true;true;true;true;true;true;true;true;true;true;true].
+
+(* trace_tf_count-3 *)
+Definition trace_tf_count_3 : list bool :=
+  [false;false;false;false;false;false;false;false;false;false;false;false;false;false;false;false].
+
+(* trace_tf_count-4 *)
+Definition trace_tf_count_4 : list bool :=
+  [false;true;false;true;false;true;false;true;false;true;false;true;false;true;false;true].
+
+(* trace_tf_count-5 *)
+Definition trace_tf_count_5 : list bool :=
+  [false;true;false;true;false;true;false;true;false;false;false;false;true;true;true;true].
+
+(** ** Signed integer traces
+*)
+Definition trace_int_1 : list Z :=
+  [1%Z;2%Z;3%Z;4%Z;5%Z;6%Z;7%Z;8%Z;9%Z;10%Z;11%Z;12%Z;13%Z;14%Z;15%Z;16%Z].
+
+Definition trace_int_2 : list Z :=
+  [0%Z;0%Z;0%Z;0%Z;0%Z;0%Z;0%Z;0%Z;0%Z;0%Z;0%Z;1%Z;2%Z;3%Z;4%Z;4%Z].
+
+Definition trace_int_3 : list Z :=
+  [0%Z;1%Z;2%Z;3%Z;2%Z;1%Z;0%Z;1%Z;2%Z;3%Z;2%Z;1%Z;0%Z;1%Z;2%Z;3%Z].
+
+Definition trace_int_4 : list Z :=
+  [0%Z;0%Z;0%Z;0%Z;1%Z;1%Z;1%Z;2%Z;3%Z;4%Z;4%Z;4%Z;4%Z;4%Z;4%Z;4%Z].
+
+(* slightly extended trace_abs-1 *)
+Definition trace_abs : list Z :=
+  [1%Z;2%Z;3%Z;(-1)%Z;(-2)%Z;(-3)%Z;4%Z;5%Z;6%Z;(-4)%Z;(-5)%Z;(-6)%Z;7%Z;8%Z;(-7)%Z;(-8)%Z].
